### Golden Ratio
---
Two quantities `a` and `b` are said to be in the Golden ratio if `(a+b)/a = a/b = ϕ`

`ϕ` has the property that `ϕ^2 = 1 + ϕ` as

```
	(a + b)/a = ϕ
	1 + b/a = ϕ
	1 + 1/ϕ = ϕ
	ϕ + 1 = ϕ^2
```

Solving `ϕ^2 -ϕ -1 = 0`, we get

`([1+√5]/2)([1-√5]/2) = 0`

Let `ψ = [1-√5]/2`. Similarly, `ψ` also has the property `ψ^2 = 1 + ψ`

### Fibonacci Definition
---
The definition of the Fibonacci sequence is

```
           { 0                     if n = 0		   
Fib(n) =   { 1                     if n = 1
           { (Fib(n-1) + Fib(n-2)  otherwise
```

### Proof by strong Induction
---

Let `P(n)` be the statement that `Fib(n) = (ϕ^n - ψ^n)/√5`

```
For n = 0, Fib(0) = (ϕ^0 - ψ^0)/√5
                  = (1 - 1)/√5
                  = 0
so, P(0) is true

For n = 1, Fib(1) = (ϕ^1 - ψ^1)/√5
                  = (ϕ - ψ)/√5
                  = ([1+√5]/2 - [1-√5]/2) / √5
				  = [1/2 (1+√5-1+√5)] / √5
				  = [1/2 (2√5)] / √5
				  = √5 / √5
				  = 1
so, P(1) is true
```

Now, suppose that `P(2), ..., P(n)`, are true for all positive integers n, that is, for `Fib(k) = (ϕ^k - ψ^k)/√5`

```
Then P(k) + P(k-1) = (ϕ^k - ψ^k)/√5 + (ϕ^k-1 - ψ^k-1)/√5
                   = 1//√5[ ϕ^k - ψ^k + ϕ^k-1 - ψ^k-1]
				   = 1//√5[ ϕ^k-1(1+ϕ) - ψ^k-1(1+ψ)]
				   = 1//√5[ (ϕ^k-1)ϕ^2 - (ψ^k-1)ψ^2] from the properties of the Golden Ratio above
				   = [ϕ^k+1 - ψ^k+1] /√5
				   = P(k+1)
				   
So P(k+1) is true.
```

Since we have shown that `P(0)`, and `P(1)` are true, and that `P(0), ... , P(k)` together imply `P(k+1)`, it follows 
that `P(n)` is true for integers `n` that are greater than or equal to zero.

Hence `Fib(n) = (ϕ^n - ψ^n)/√5`, where `ϕ = [1+√5]/2` and `ψ = [1-√5]/2`

### Final simplification
---
Given that `Fib(n) = (ϕ^n - ψ^n)/√5` and `ψ = [1-√5]/2`, we can note that `ψ = [1-√5]/2` is less than 1, so will tend to zero as `n` increases.

At it's largest, for `n = 0`, `ψ = 1/√5` which is `< 0.5`, therefore `Fib(n)` is the closest integer to `ϕ^n/√5`

